Rename file containing state passing MST

experiments/dm4ms/Bad_State_Passing.fst
@@ -1,7 +1,70 @@
-module TOTAL_MST2
+module Bad_State_Passing
 
-open WMonad
+let st_pre_h (heap: Type) = heap -> GTot Type0
 
+(** Postconditions relate [a]-typed results to the final [heap], here
+    refined by some pure proposition [pre], typically instantiated to
+    the precondition applied to the initial [heap] *)
+let st_post_h' (heap a pre: Type) = a -> _: heap{pre} -> GTot Type0
+
+(** Postconditions without refinements *)
+let st_post_h (heap a: Type) = st_post_h' heap a True
+
+unfold
+let st_post_ord (#heap:Type) (p1 p2:st_post_h heap 'a) =
+  forall r h. p1 r h ==> p2 r h
+
+(** The type of the main WP-transformer for stateful computations *)
+let st_wp_h (heap a: Type) = st_post_h heap a -> Tot (st_pre_h heap)
+
+(** Returning a value does not transform the state *)
+unfold
+let st_return (heap:Type u#b) (a: Type u#a) (x: a) (p: st_post_h heap a) = p x
+
+(** Sequential composition of stateful WPs *)
+unfold
+let st_bind_wp
+      (heap: Type u#c)
+      (a:Type u#a)
+      (b: Type u#b)
+      (wp1: st_wp_h heap a)
+      (wp2: (a -> GTot (st_wp_h heap b)))
+      (p: st_post_h heap b)
+      (h0: heap)
+     = wp1 (fun a h1 -> wp2 a p h1) h0
+
+(** Branching for stateful WPs *)
+unfold
+let st_if_then_else
+      (heap a p: Type)
+      (wp_then wp_else: st_wp_h heap a)
+      (post: st_post_h heap a)
+      (h0: heap)
+     = wp_then post h0 /\ (~p ==> wp_else post h0)
+
+(** As with [PURE] the [wp] combinator names the postcondition as
+    [k] to avoid duplicating it. *)
+unfold
+let st_ite_wp (heap a: Type) (wp: st_wp_h heap a) (post: st_post_h heap a) (h0: heap) =
+  forall (k: st_post_h heap a).
+    (forall (x: a) (h: heap). {:pattern (guard_free (k x h))} post x h ==> k x h) ==> wp k h0
+
+(** Subsumption for stateful WPs *)
+unfold
+let st_stronger (heap a: Type) (wp1 wp2: st_wp_h heap a) =
+  (forall (p: st_post_h heap a) (h: heap). wp1 p h ==> wp2 p h)
+
+unfold
+let (⊑) #heap #a wp1 wp2 = st_stronger heap a wp2 wp1
+
+(** Closing the scope of a binder within a stateful WP *)
+unfold
+let st_close_wp (heap a b: Type) (wp: (b -> GTot (st_wp_h heap a))) (p: st_post_h heap a) (h: heap) =
+  (forall (b: b). wp b p h)
+
+(** Applying a stateful WP to a trivial postcondition *)
+unfold
+let st_trivial (heap a: Type) (wp: st_wp_h heap a) = (forall h0. wp (fun r h1 -> True) h0)
 
 open FStar.Tactics
 module W = FStar.Monotonic.Witnessed
@@ -126,6 +189,6 @@ let test () : mst nat_state int (fun p h0 -> forall r h1. p r h1) =
       `mst_bind`
       (fun () ->
         (fun hi -> (** here I directly use the state monad *)
-          let (_, r) = f () 0 in (** I can call f with state 0.
+          let (_, r) = f () 0 in (** BROKEN!!!! I can call f with state 0.
                ^ we cannot return this state because it is not greater than h0 *)
           (hi, r)) <: mst nat_state int (fun p h -> (forall r. p r h)))))
